stash progress

src/examples/simple-prot.v
@@ -1,29 +1,78 @@
 From iris.proofmode Require Import tactics.
 From iris.bi Require Import monpred.
+From iris.program_logic Require weakestpre.
 
 From self.base Require Import primitive_laws.
 From self.lang Require Import lang.
 From self.high Require Import dprop.
 
-From self.lang Require Import notation lang.
+From self.lang Require Export notation lang lemmas tactics syntax.
 From self.algebra Require Import view.
 From self.base Require Import primitive_laws class_instances adequacy.
 From self.high Require Import proofmode wpc_proofmode.
-From self.high Require Import weakestpre_exp weakestpre_at.
+From self.high Require Import weakestpre_exp locations.
+From self.high.modalities Require Import fence.
 From self.high Require Import protocol no_buffer abstract_state_instances.
+
+Section Axioms.
+  Context `{AbstractState ST}.
+  Context `{!nvmG Σ}.
+
+  Implicit Types (ℓ : loc) (s : ST) (prot : LocationProtocol ST).
+
+  Lemma wp_store_na ℓ prot (ss: list ST) v s__last s st E `{!ProtocolConditions prot} :
+    list.last ss = Some s__last →
+    s__last ⊑ s →
+    {{{ mapsto_na ℓ prot 1 ss ∗ prot.(p_full) s v }}}
+      #ℓ <-_NA v @ st; E
+    {{{ RET #(); mapsto_na ℓ prot 1 (ss ++ [s]) }}}.
+  Proof.
+  Admitted.
+
+
+  Lemma wp_cmpxchg_at Q1 Q2 Q3 ℓ prot `{!ProtocolConditions prot} ss s_i (v_i : val) v_t R s_t st E :
+    {{{
+      ℓ ↦_AT^{prot} (ss ++ [s_i]) ∗
+      (∀ s_l v_l s_p v_p, ∃ P, ⌜ s_i ⊑ s_l ⌝ -∗
+        ((▷ prot.(p_read) s_l v_l) -∗ ⌜ vals_compare_safe v_i v_l ⌝) ∗
+        (( (* in case of success *)
+            ⌜ v_l = v_i ⌝ -∗
+            (* The state we write fits in the history. *)
+            (<obj> (prot.(p_full) s_l v_l -∗ ⌜ s_l ⊑ s_t ⌝)) ∗
+            (∀ s_n v_n, ⌜ s_l ⊑ s_n ⌝ -∗ prot.(p_full) s_l v_l -∗
+                        prot.(p_read) s_n v_n -∗ ⌜ s_l = s_n ∨ s_t ⊑ s_n ⌝) ∗
+            (* Extract the objective knowledge from [p_pers] *)
+            (<obj> (prot.(p_pers) s_p v_p -∗ <obj> P ∗ (P -∗ prot.(p_pers) s_p v_p))) ∗
+            (* Extract from the location we load. *)
+            (<obj> (prot.(p_full) s_l v_l ∗ P -∗ prot.(p_read) s_l v_l ∗ R s_l)) ∗
+            (* Establish the invariant for the value we store. *)
+            (R s_l ==∗ prot.(p_full) s_t v_t ∗ <obj> P ∗ Q1 s_l))
+         ∧ (* in case of failure *)
+           ((<obj> (prot.(p_full) s_l v_l -∗ prot.(p_full) s_l v_l ∗ Q2 s_l)) ∗ Q3)
+        ))
+    }}}
+      CmpXchg #ℓ v_i v_t @ st; E
+    {{{ v b s_l, RET (v, #b);
+      (⌜ b = true ⌝ ∗ <fence> Q1 s_l ∗ ℓ ↦_AT^{prot} ((ss ++ [s_i]) ++ [s_t])) ∨
+      (⌜ b = false ⌝ ∗ ⌜ s_i ⊑ s_l ⌝ ∗ ℓ ↦_AT^{prot} (ss ++ [s_i]) ∗ <fence> (Q2 s_l) ∗ Q3)
+    }}}.
+  Proof.
+  Admitted.
+End Axioms.
 
 Section fence_sync.
   Context `{!nvmG Σ}.
 
   Variable (ℓ ℓ': loc).
 
-
   Definition prog_left : expr :=
     #ℓ' <-_NA #42;;
-    Flush #ℓ';;
-    CmpXchg #ℓ #0 #1;;
-    Flush #ℓ;;
-    Fence #ℓ.
+    Flush #ℓ' ;;
+    Fence ;;
+    let: "b" := Snd (CmpXchg #ℓ #0 #1) in
+    Flush #ℓ ;;
+    FenceSync ;;
+    "b".
 
   Definition prog_right : expr :=
     CmpXchg #ℓ #1 #2.
@@ -32,7 +81,7 @@ Section fence_sync.
   Definition prot' : LocationProtocol nat :=
     {| p_full := λ (n : nat) v, ⌜ v = #n ⌝%I;
        p_read := λ (n : nat) v, ⌜ v = #n ⌝%I;
-       p_pers := λ (n : nat) v, ⌜ v = #n ⌝%I;
+       p_pers := λ (n : nat) v, True%I;
        p_bumper n := n |}.
 
   Global Instance prot_cond' : ProtocolConditions prot'.
@@ -58,9 +107,9 @@ Section fence_sync.
 
   (* Predicate used for the location [ℓ]. *)
   Definition prot : LocationProtocol nat :=
-    {| p_full := λ (n : nat) v, (⌜ v = #n ⌝ ∗ (⌜ n ≥ 1 ⌝ -∗ store_lb ℓ' prot' 42)) %I;
+    {| p_full := λ (n : nat) v, (⌜ v = #n ⌝ ∗ (⌜ n ≥ 1 ⌝ -∗ store_lb ℓ' prot' 42 ∗ flush_lb ℓ' prot' 42)) %I;
        p_read := λ (n : nat) v, ⌜ v = #n ⌝%I;
-       p_pers := λ (n : nat) v, (⌜ v = #n ⌝ ∗ (⌜ n ≥ 1 ⌝ -∗ flush_lb ℓ' prot' 42))%I;
+       p_pers := λ (n : nat) v, True%I;
        p_bumper n := n |}.
 
   Global Instance prot_cond : ProtocolConditions prot.
@@ -68,17 +117,6 @@ Section fence_sync.
     split; try apply _.
     { intros.
       rewrite /IntoNoBuffer /p_full /prot //=.
-      iIntros "[% H]".
-      destruct (decide (1 ≤ s)).
-      - iSpecialize ("H" with "[//]").
-        iModIntro.
-        iSplit; first done.
-        by iIntros.
-      - iModIntro.
-        iSplit; first done.
-        iIntros; lia. }
-    { intros.
-      rewrite /IntoNoBuffer /p_pers /prot //=.
       iIntros "[% H]".
       destruct (decide (1 ≤ s)).
       - iSpecialize ("H" with "[//]").
@@ -97,64 +135,200 @@ Section fence_sync.
         by iApply "H".  }
   Admitted.
 
-  Lemma spec_right st E:
-    {{{ ℓ ↦_AT^{prot} [0] }}}
-      prog_right @ st; E
-      {{{ v b, RET (v, #b); ⌜ b = true ⌝ -∗ store_lb ℓ' prot' 42 }}}.
+  Lemma spec_left st E:
+    {{{ ℓ' ↦_{prot'} [0] ∗ ℓ ↦_AT^{prot} [0] }}}
+      prog_left @ st; E
+    {{{ b, RET #b; ⌜b = true⌝ -∗ persist_lb ℓ prot 1 }}}.
   Proof.
-    iIntros (Φ) "pts Φpost".
-    rewrite /prog_right.
+    iIntros (Φ) "[pts' pts] Φpost".
+    rewrite /prog_left.
+    wp_apply (wp_store_na _ prot' [0] _ _ 42 with "[pts']");
+      [ done | rewrite /sqsubseteq //=; lia | by iFrame | ].
+    rewrite //=. iIntros "pts'".
+    wp_pures.
+    wp_apply (weakestpre.wp_flush_na _ prot' 42 1%Qp [0] with "pts'").
+    iIntros "(pts' & #flush_lb' & _)".
+    wp_pures.
+    wp_apply (weakestpre.wp_fence).
+    do 2 iModIntro.
+    wp_pures.
     wp_apply (wp_cmpxchg_at
-                (λ n, ⌜n = 1⌝ -∗ store_lb ℓ' prot' 42)%I
+                (λ n, True)%I
                 (λ _, True)%I
                 (True)%I
                 ℓ prot [] 0 _ _
-                (λ n, ⌜n = 1⌝ -∗ store_lb ℓ' prot' 42)%I
-                2 with "[$pts]").
+                (λ n, True)%I
+                1 with "[$pts pts']").
     { iIntros.
       iExists (True)%I.
       iIntros.
-      iSplit.
       (* safe comparison *)
-      { admit. }
+      iSplit. { iIntros "_". iPureIntro. left. done. }
       iSplit.
       (* success *)
       { iIntros.
         subst.
         rewrite /p_full /p_read /p_pers /prot //=.
         iSplitL "".
-        - iIntros "!>[% H]".
+        { iIntros "!>[% H]".
           simplify_eq.
           iPureIntro.
           rewrite /sqsubseteq.
-          lia.
-        -
+          lia. }
+        iSplitL "".
+        { rewrite /sqsubseteq.
+          iIntros (??) "% [% ?] %".
+          simplify_eq.
+          iPureIntro.
+          lia. }
+        iSplitL "".
+        { iIntros "!> _".
+          iSplitL ""; first by iModIntro.
+          done. }
+        iSplitL "".
+        { iIntros "!>[[% φ_old] _]".
+          iFrame "%". }
+        iIntros "_ !>".
+        iPoseProof (mapsto_na_store_lb ℓ' prot' (1%Qp) [0] 42 with "pts'") as "#?".
+        iFrame "#".
+        iSplitPure; first done.
+        iSplit; first iModIntro; done.
       }
-    }
+      (* failure *)
+      { iSplit; last done.
+        iIntros "!> ?".
+        iFrame. } }
+    iIntros (???) "[H | H]"; rewrite //=.
+    - (* successful *)
+      wp_pures.
+      wp_apply (wp_flush_lb _ prot 1 _ _ True%I with "[H]").
+      { iDestruct "H" as "(_ & _ & H)".
+        iSplit; first iApply (mapsto_at_store_lb ℓ prot [0] with "[$]").
+        iSplit.
+        { rewrite /mapsto_at.
+          iNamed "H".
+          done. }
+        rewrite /R_progress.
+        iModIntro.
+        iIntros.
+        iExists True%I, True%I.
+        iSplitL "".
+        { iIntros. repeat iModIntro. done. }
+        iSplitL "".
+        { iIntros. repeat iModIntro. done. }
+        iIntros.
+        iSplit.
+        { iIntros "_ !>". done. }
+        done. }
+      iIntros "post_fence".
+      wp_pures.
+      wp_apply (wp_fence_sync with "post_fence").
+      iIntros "[? _]".
+      wp_pures.
+      iModIntro.
+      iApply "Φpost".
+      iFrame.
+      done.
+    - (* failed *)
+      (* probably better have a lemma for flush that's essentially no-op *)
+      wp_pures.
+      iDestruct "H" as "(% & % & H & _)".
+      wp_apply (wp_flush_lb _ prot 0 _ _ True%I with "[H]").
+      { iSplit; first iApply (mapsto_at_store_lb ℓ prot [] with "[$]").
+        iSplit.
+        { rewrite /mapsto_at.
+          iNamed "H".
+          done. }
+        rewrite /R_progress.
+        iModIntro.
+        iIntros.
+        iExists True%I, True%I.
+        iSplitL "".
+        { iIntros. repeat iModIntro. done. }
+        iSplitL "".
+        { iIntros. repeat iModIntro. done. }
+        iIntros.
+        iSplit.
+        { iIntros "_ !>". done. }
+        done. }
+      iIntros "post_fence".
+      wp_pures.
+      wp_apply (wp_fence_sync with "post_fence").
+      iIntros "[? _]".
+      wp_pures.
+      iModIntro.
+      iApply "Φpost".
+      iIntros "%".
+      congruence.
+  Qed.
 
-  Lemma spec ℓ st E :
-    {{{ ℓ ↦_{prot} [0] }}}
-      program ℓ @ st; E
-    {{{ RET #(); ℓ ↦_{prot} [1] }}}.
+  Lemma spec_right st E:
+    {{{ ℓ ↦_AT^{prot} [0] }}}
+      prog_right @ st; E
+      {{{ v b, RET (v, #b); ⌜ b = true ⌝ -∗ <fence> store_lb ℓ' prot' 42 }}}.
   Proof.
     iIntros (Φ) "pts Φpost".
-    rewrite /program.
-    wp_apply (wp_store_na with "[$pts]"); first done.
-    { suff leq : (0 ≤ 1); first apply leq. lia. }
-    { done. }
-    iIntros "pts".
-    wp_pures.
-    wp_apply (wp_flush_na with "pts").
-    iIntros "(pts & _ & lb) /=".
-    wp_pures.
-    wp_apply wp_fence_sync.
-    iModIntro.
-    simpl.
-    wp_pures.
-    iModIntro.
+    rewrite /prog_right.
+    wp_apply (wp_cmpxchg_at
+                (λ n, ⌜1%Z = Z.of_nat n⌝ ∗ store_lb ℓ' prot' 42)%I
+                (λ _, True)%I
+                (True)%I
+                ℓ prot [] 0 _ _
+                (λ n, ⌜1%Z = Z.of_nat n⌝ ∗ store_lb ℓ' prot' 42)%I
+                2 with "[$pts]").
+    { iIntros.
+      iExists (True)%I.
+      iIntros.
+      (* safe comparison *)
+      iSplit. { iIntros "_". iPureIntro. left. done. }
+      iSplit.
+      (* success *)
+      { iIntros.
+        subst.
+        rewrite /p_full /p_read /p_pers /prot //=.
+        iSplitL "".
+        { iIntros "!>[% H]".
+          simplify_eq.
+          iPureIntro.
+          rewrite /sqsubseteq.
+          lia. }
+        iSplitL "".
+        { rewrite /sqsubseteq.
+          iIntros (??) "% [% ?] %".
+          simplify_eq.
+          iPureIntro.
+          lia. }
+        iSplitL "".
+        { iIntros "!>[% ?]".
+          iSplitL ""; first by iModIntro.
+          iIntros "_".
+          iFrame "%".
+          done. }
+        iSplitL "".
+        { iIntros "!>[[% φ_old] _]".
+          iFrame "%".
+          simplify_eq.
+          iFrame "%".
+          iApply "φ_old".
+          iPureIntro.
+          lia. }
+        iIntros "[% #?] !>".
+        iFrame "#%".
+        iSplit; last by iModIntro.
+        iSplitPure; first done.
+        by iIntros.
+      }
+      (* failure *)
+      { iSplit; last done.
+        iIntros "!> ?".
+        iFrame. } }
+    iIntros (???) "H".
     iApply "Φpost".
-    iApply (mapsto_na_persist_lb with "pts lb").
-    cbn. lia.
+    iIntros.
+    iDestruct "H" as "[ (_ & [? ?] & _) | [% _] ]"; last congruence.
+    iFrame.
   Qed.
+
+  Lemma
 
 End fence_sync.
